Some sketches on action types

theories/Pi/Control.v
@@ -13,28 +13,31 @@ Require Import Local.Pi.Calculus.
 
 Set Primitive Projections.
 
-Record env: Set := {
+Notation nodes := (list (option type)).
+
+Record env: Type := env_mk {
   env_nodes:
-    list (option type);
+    nodes;
   env_edges:
-    list (nat * nat)
+    relation nat
 }.
 
 Global Coercion env_nodes: env >-> list.
 
-Definition env_adjacency (g: env): relation nat :=
-  fun x y =>
-    In (x, y) (env_edges g).
+Definition env_empty: env := {|
+  env_nodes := [];
+  env_edges x y := False
+|}.
 
 Record env_wellformed (g: env): Prop := {
   env_wellformed_domain:
     forall i j,
-    env_adjacency g i j ->
+    env_edges g i j ->
     exists ts,
     nth i g None = Some (channel I ts);
   env_wellformed_codomain:
     forall i j,
-    env_adjacency g i j ->
+    env_edges g i j ->
     exists ts,
     nth j g None = Some (channel O ts)
 }.
@@ -63,16 +66,24 @@ Definition type_coherent: relation type :=
   fun t1 t2 =>
     exists t3, type_composition t1 t2 t3.
 
+Lemma type_composition_sym:
+  forall t1 t2 t3,
+  type_composition t1 t2 t3 ->
+  type_composition t2 t1 t3.
+Proof.
+  destruct 1; subst.
+  - now apply type_composition_io with ts.
+  - now apply type_composition_oi with ts.
+  - now apply type_composition_oo with ts.
+Qed.
+
 Lemma type_coherent_sym:
   symmetric type_coherent.
 Proof.
   intros t1 t2 ?.
   destruct H as (t3, ?).
   exists t3.
-  dependent destruction H; subst.
-  - now apply type_composition_io with ts.
-  - now apply type_composition_oi with ts.
-  - now apply type_composition_oo with ts.
+  now apply type_composition_sym.
 Qed.
 
 Record env_coherent (g: env) (h: env): Prop := {
@@ -81,4 +92,205 @@ Record env_coherent (g: env) (h: env): Prop := {
     nth i g None = Some t1 ->
     nth i h None = Some t2 ->
     type_coherent t1 t2;
+  env_coherent_acyclic:
+    well_founded (union (env_edges g) (env_edges h))
 }.
+
+Inductive env_composition_nodes: nodes -> nodes -> nodes -> Prop :=
+  | env_composition_nodes_nil_left:
+    forall h,
+    env_composition_nodes [] h h
+  | env_composition_nodes_nil_right:
+    forall g,
+    env_composition_nodes g [] g
+  | env_composition_nodes_cons_left:
+    forall g h i t,
+    env_composition_nodes g h i ->
+    env_composition_nodes (t :: g) (None :: h) (t :: i)
+  | env_composition_nodes_cons_right:
+    forall g h i t,
+    env_composition_nodes g h i ->
+    env_composition_nodes (None :: g) (t :: h) (t :: i)
+  | env_composition_nodes_cons_compose:
+    forall g h i t1 t2 t3,
+    env_composition_nodes g h i ->
+    type_composition t1 t2 t3 ->
+    env_composition_nodes (Some t1 :: g) (Some t2 :: h) (Some t3 :: i).
+
+Definition lower_bound i (R: relation nat): Prop :=
+  forall j, ~R j i.
+
+Definition upper_bound i (R: relation nat): Prop :=
+  forall j, ~R i j.
+
+Inductive env_composition_edges: env -> env -> relation nat :=
+  | env_composition_edges_mk:
+    forall g h,
+    let x := union (env_edges g) (env_edges h) in
+    forall i j,
+    x i j ->
+    lower_bound i x ->
+    upper_bound j x ->
+    env_composition_edges g h i j.
+
+Inductive env_composition: env -> env -> env -> Prop :=
+  | env_composition_mk:
+    forall g: env,
+    forall h: env,
+    forall i: nodes,
+    env_composition_nodes g h i ->
+    env_composition g h (env_mk i (env_composition_edges g h)).
+
+Goal
+  forall g h,
+  env_coherent g h ->
+  exists i,
+  env_composition g h i.
+Proof.
+  destruct 1 as (?H, ?H).
+  assert (exists i, env_composition_nodes g h i) as (i, ?).
+  - clear H0.
+    destruct g as (g, R).
+    destruct h as (h, S).
+    simpl in H |- *.
+    clear R S.
+    generalize dependent h.
+    induction g; intros.
+    + eexists; constructor.
+    + destruct h.
+      * eexists; constructor.
+      * destruct IHg with h as (i, ?); intros.
+        --- apply H with (S i); now simpl.
+        --- destruct a, o.
+            +++ destruct H with 0 t t0 as (?t, ?); simpl; auto.
+                eexists; constructor.
+                *** eassumption.
+                *** eassumption.
+            +++ eexists; constructor.
+                eassumption.
+            +++ eexists; constructor.
+                eassumption.
+            +++ eexists; constructor.
+                eassumption.
+  - eexists.
+    constructor.
+    eassumption.
+Qed.
+
+Definition env_equiv (g h: env): Prop :=
+  env_nodes g = env_nodes h /\ same_relation (env_edges g) (env_edges h).
+
+Lemma env_equiv_refl:
+  reflexive env_equiv.
+Proof.
+  split; intros.
+  - reflexivity.
+  - firstorder.
+Qed.
+
+Lemma env_equiv_sym:
+  symmetric env_equiv.
+Proof.
+  destruct 1; split.
+  - auto.
+  - destruct H0; firstorder.
+Qed.
+
+Lemma env_equiv_trans:
+  transitive env_equiv.
+Proof.
+  destruct 1, 1; split.
+  - now transitivity y.
+  - destruct H0; destruct H2; firstorder.
+Qed.
+
+Lemma env_composition_nodes_sym:
+  forall g h i,
+  env_composition_nodes g h i ->
+  env_composition_nodes h g i.
+Proof.
+  induction 1.
+  - constructor.
+  - constructor.
+  - now constructor.
+  - now constructor.
+  - constructor.
+    + assumption.
+    + now apply type_composition_sym.
+Qed.
+
+Lemma env_composition_edges_switch:
+  forall g h,
+  inclusion (env_composition_edges g h) (env_composition_edges h g).
+Proof.
+  intros g h x y ?.
+  dependent destruction H; constructor.
+  - destruct H; firstorder.
+  - intros z ?.
+    apply H0 with z.
+    destruct H2; firstorder.
+  - intros z ?.
+    apply H1 with z.
+    destruct H2; firstorder.
+Qed.
+
+Lemma env_composition_sym:
+  forall g h i1,
+  env_composition g h i1 ->
+  exists2 i2,
+  (* We don't have propositional extensionality... *)
+  env_composition h g i2 & env_equiv i1 i2.
+Proof.
+  destruct 1; simpl.
+  apply env_composition_nodes_sym in H.
+  eexists.
+  - constructor.
+    eassumption.
+  - split; simpl.
+    + reflexivity.
+    + split; intros x y ?.
+      * now apply env_composition_edges_switch.
+      * now apply env_composition_edges_switch.
+Qed.
+
+Lemma env_composition_unit_left:
+  forall g,
+  exists2 h,
+  env_composition env_empty g h & env_equiv g h.
+Proof.
+  intros.
+  eexists (env_mk g _).
+  - constructor; simpl.
+    destruct g as (g, R).
+    simpl; clear R.
+    induction g.
+    + constructor.
+    + constructor.
+  - constructor; simpl.
+    + reflexivity.
+    + split; intros x y ?.
+      * constructor.
+        --- now right.
+        --- (* Hmm... *)
+            admit.
+        --- (* Oh, well... *)
+            admit.
+      * dependent destruction H.
+        destruct H; simpl in *.
+        --- exfalso.
+            contradiction.
+        --- assumption.
+Admitted.
+
+Lemma env_composition_unit_right:
+  forall g,
+  exists2 h,
+  env_composition g env_empty h & env_equiv g h.
+Proof.
+  intros.
+  destruct env_composition_unit_left with g as (h, ?, ?).
+  destruct env_composition_sym with env_empty g h as (i, ?, ?); auto.
+  exists i.
+  - assumption.
+  - now apply env_equiv_trans with h.
+Qed.
